matching-logic/src/Theories/Definedness_ProofSystem.v
@@ -3149,64 +3149,121 @@ Proof.
     mgRewrite <- H at 1. mgIntro. mgExactn 0.
 Defined.
 
-Lemma ceil_monotonic_obj {Σ : Signature} {syntax : Syntax} Γ ϕ₁ ϕ₂ :
-theory ⊆ Γ ->
-well_formed ϕ₁ ->
-well_formed ϕ₂ ->
-Γ ⊢ (ϕ₁ ---> ϕ₂) ---> ⌈ ϕ₁ ⌉ ---> ⌈ ϕ₂ ⌉.
-Proof. Search patt_total ML_proof_system.
-  (* intros HΓ Wf1 Wf2.
-  toMyGoal. wf_auto2.
-  pose proof (@impl_iff_notp_or_q _ Γ ϕ₁ ϕ₂ Wf1 Wf2).
-  mgRewrite H at 1.
-  pose proof (@impl_iff_notp_or_q _ Γ ⌈ϕ₁⌉ ⌈ϕ₂⌉ ltac:(wf_auto2) ltac:(wf_auto2)).
-  mgRewrite H0 at 1.
-  Search patt_defined patt_imp.
+Lemma patt_or_total {Σ : Signature} {syntax : Syntax}:
+  forall Γ φ ψ,
+  theory ⊆ Γ ->
+  well_formed φ -> well_formed ψ ->
+  Γ ⊢  ⌊ φ ⌋ or ⌊ ψ ⌋ ---> ⌊ φ or ψ ⌋.
+Proof.
+  intros Γ φ ψ HΓ Wf1 Wf2. toMyGoal. wf_auto2.
   mgIntro. mgDestructOr 0.
-  * mgLeft. mgIntro. mgApply 0.
-  
+  * pose proof (@disj_left_intro _ Γ φ ψ Wf1 Wf2) as H.
+    apply floor_monotonic in H. 2-4: try wf_auto2.
+    mgApplyMeta H. mgExactn 0.
+  * pose proof (@disj_right_intro _ Γ φ ψ Wf1 Wf2) as H.
+    apply floor_monotonic in H. 2-4: try wf_auto2.
+    mgApplyMeta H. mgExactn 0.
+Defined.
 
-  mgAssert ((⌈ ϕ₁ ---> ϕ₂ ⌉)). wf_auto2.
-  mgApplyMeta (@phi_impl_defined_phi _ _ Γ (ϕ₁ ---> ϕ₂) HΓ ltac:(wf_auto2)).
-  mgExactn 0. mgClear 0.
-  mgIntro. Search "cong" patt_iff.
-  Check (@P4 _ Γ (⌈ ϕ₁ ⌉ ---> ⌈ ϕ₂ ⌉) _ ltac:(wf_auto2) Hwf).
-  pose proof (@impl_iff_notp_or_q _ Γ ⌈ϕ₁⌉ ⌈ϕ₂⌉ ltac:(wf_auto2) ltac:(wf_auto2)).
-  Search patt_imp ML_proof_system.
-  
-  apply pf_iff_proj2 in H. 2-3: wf_auto2.
-  mgRevert. mgApplyMeta H.
-  Search patt_total. Print patt_defined.
-  pose proof (@impl_iff_notp_or_q _ Γ ϕ₁ ϕ₂ Wf1 Wf2).
-  mgRevert.
-  (* mgRewrite H0 at 2. <- TODO: does not work! *)
-  Search "cong" patt_iff.
-  Print PatternCtx.
-  Search fresh_evar.
-  remember ({| pcEvar    := fresh_evar (ϕ₁ ---> ϕ₂);
-           pcPattern := ⌈ patt_free_evar (fresh_evar (ϕ₁ ---> ϕ₂)) ⌉ 
-                         ---> ! ⌈ ϕ₁ ⌉ or ⌈ ϕ₂ ⌉ |}) as C.
-  epose proof (@prf_equiv_congruence _ Γ (ϕ₁ ---> ϕ₂) (! ϕ₁ or ϕ₂) C ltac:(wf_auto2) H0).
-  apply pf_iff_proj2 in H1. 2-3: rewrite HeqC; wf_auto2; case_match; wf_auto2.
-  rewrite HeqC in H1. cbn in H1. case_match. 2: congruence.
-  Search free_evar_subst.
-  repeat rewrite free_evar_subst_no_occurrence in H1.
-  1-4: apply count_evar_occurrences_0; eapply evar_is_fresh_in_richer';
-      [ |apply set_evar_fresh_is_fresh'];
-      solve_free_evars_inclusion 5.
-  mgApplyMeta H1.
-  replace (patt_sym (Definedness_Syntax.inj definedness) $ (! ϕ₁ or ϕ₂)) with
-          (⌈! ϕ₁ or ϕ₂ ⌉) by auto.
-  replace (((patt_sym (Definedness_Syntax.inj definedness) $ ϕ₁ ---> ⊥) ---> ⊥) --->
-patt_sym (Definedness_Syntax.inj definedness) $ ϕ₂) with (! ⌈ ϕ₁ ⌉ or ⌈ ϕ₂ ⌉) by auto.
-  clear H1 HeqC Heqs C e.
-  mgIntro. mgAssert ((⌈ ! ϕ₁ ⌉ or ⌈ ϕ₂ ⌉)). wf_auto2.
-  pose proof (Prop_disj_right Γ (! ϕ₁) ϕ₂ (patt_sym (Definedness_Syntax.inj definedness)) ltac:(wf_auto2) Wf2 ltac:(wf_auto2)).
-  mgApplyMeta H1. mgExactn 0.
-  mgClear 0.
+Lemma patt_defined_and {Σ : Signature} {syntax : Syntax}:
+  forall Γ φ ψ,
+  theory ⊆ Γ ->
+  well_formed φ -> well_formed ψ ->
+  Γ ⊢ ⌈ φ and ψ ⌉ ---> ⌈ φ ⌉ and ⌈ ψ ⌉.
+Proof.
+  intros Γ φ ψ HΓ Wf1 Wf2. toMyGoal. wf_auto2.
+  unfold patt_and.
+  mgRewrite (@defined_not_iff_not_total _ _ Γ (! φ or ! ψ) HΓ ltac:(wf_auto2)) at 1.
+  do 2 mgIntro. mgApply 0. mgClear 0.
+  mgApplyMeta (@patt_or_total _ _ _ (! φ) (! ψ) HΓ ltac:(wf_auto2) ltac:(wf_auto2)).
   mgDestructOr 0.
-  * mgLeft. Search patt_defined ML_proof_system.
-  * mgRight. mgExactn 0.
-  Unshelve.
-  rewrite HeqC. unfold PC_wf. wf_auto2. *)
-Abort.
+  * mgLeft. unfold patt_total.
+    mgRewrite <- (@not_not_iff _ Γ φ Wf1) at 1. mgExactn 0.
+  * mgRight. unfold patt_total.
+    mgRewrite <- (@not_not_iff _ Γ ψ Wf2) at 1. mgExactn 0.
+Defined.
+
+Lemma patt_total_and {Σ : Signature} {syntax : Syntax}:
+  forall Γ φ ψ,
+  theory ⊆ Γ ->
+  well_formed φ -> well_formed ψ ->
+  Γ ⊢ ⌊ φ and ψ ⌋ <---> ⌊ φ ⌋ and ⌊ ψ ⌋.
+Proof.
+  intros Γ φ ψ HΓ Wf1 Wf2. toMyGoal. wf_auto2.
+  mgSplitAnd.
+  * unfold patt_and.
+    mgRewrite <- (@def_propagate_not _ _ Γ (! φ or ! ψ) HΓ ltac:(wf_auto2)) at 1.
+    mgIntro. mgIntro. mgApply 0.
+    mgClear 0.
+    mgRewrite (@ceil_compat_in_or _ _ Γ (! φ) (! ψ) HΓ ltac:(wf_auto2) ltac:(wf_auto2)) at 1.
+    mgDestructOr 0.
+    - mgLeft. mgRevert. unfold patt_total.
+      mgRewrite <- (@not_not_iff _ Γ ⌈ ! φ ⌉ ltac:(wf_auto2)) at 1.
+      mgIntro. mgExactn 0.
+    - mgRight. mgRevert. unfold patt_total.
+      mgRewrite <- (@not_not_iff _ Γ ⌈ ! ψ ⌉ ltac:(wf_auto2)) at 1.
+      mgIntro. mgExactn 0.
+  * mgIntro. mgDestructAnd 0.
+    unfold patt_and.
+    mgRewrite <- (@def_propagate_not _ _ Γ (! φ or ! ψ) HΓ ltac:(wf_auto2)) at 1.
+    mgRewrite (@ceil_compat_in_or _ _ Γ (! φ) (! ψ) HΓ ltac:(wf_auto2) ltac:(wf_auto2)) at 1.
+    mgIntro. mgDestructOr 2.
+    - mgRevert. mgExactn 0.
+    - mgRevert. mgExactn 1.
+Defined.
+
+Lemma defined_variables_equal {Σ : Signature} {syntax : Syntax} :
+  forall x y Γ,
+  theory ⊆ Γ ->
+  Γ ⊢ ⌈ patt_free_evar y and patt_free_evar x ⌉ ---> patt_free_evar y =ml patt_free_evar x.
+Proof.
+  intros x y Γ HΓ.
+  toMyGoal. wf_auto2.
+  unfold patt_equal, patt_iff.
+  pose proof (@patt_total_and _ _ _
+                                (patt_free_evar y ---> patt_free_evar x)
+                                (patt_free_evar x ---> patt_free_evar y) HΓ ltac:(wf_auto2) ltac:(wf_auto2)) as H.
+  apply pf_iff_proj2 in H. 2-3: wf_auto2.
+  mgIntro.
+  mgApplyMeta H. clear H.
+  mgIntro. mgDestructOr 1.
+  * mgApply 1. mgClear 1. mgIntro.
+    pose proof (H := @ProofMode.nimpl_eq_and _ Γ (patt_free_evar y) (patt_free_evar x)
+                  ltac:(wf_auto2) ltac:(wf_auto2)).
+    epose proof (H0 := @prf_equiv_congruence _ Γ 
+    _ _ {| pcEvar := x; pcPattern := ⌈ patt_free_evar x ⌉  |} ltac:(wf_auto2) H).
+    cbn in H0. case_match. 2: congruence.
+    apply pf_iff_proj1 in H0. 2-3: wf_auto2.
+    mgApplyMeta H0 in 1.
+    (* TODO: it is increadibly inconvienient to define concrete contexts *)
+    Check Singleton_ctx.
+    pose proof (H1 := @Singleton_ctx _ Γ 
+           (@ctx_app_r _ (patt_sym (Definedness_Syntax.inj definedness)) box 
+                ltac:(wf_auto2))
+           (@ctx_app_r _ (patt_sym (Definedness_Syntax.inj definedness)) box 
+                ltac:(wf_auto2)) (patt_free_evar x) y ltac:(wf_auto2)).
+    mgApplyMeta H1. simpl. mgSplitAnd. mgExactn 0. mgExactn 1.
+  * mgApply 1. mgClear 1. mgIntro.
+    pose proof (H := @ProofMode.nimpl_eq_and _ Γ (patt_free_evar x) (patt_free_evar y)
+                  ltac:(wf_auto2) ltac:(wf_auto2)).
+    epose proof (H0 := @prf_equiv_congruence _ Γ 
+    _ _ {| pcEvar := x; pcPattern := ⌈ patt_free_evar x ⌉  |} ltac:(wf_auto2) H).
+    cbn in H0. case_match. 2: congruence.
+    apply pf_iff_proj1 in H0. 2-3: wf_auto2.
+    mgApplyMeta H0 in 1.
+    (* TODO: mgRewriteBy does not work for free evars :( *)
+    pose proof (H1 := @patt_and_comm _ Γ (patt_free_evar y) (patt_free_evar x) ltac:(wf_auto2) ltac:(wf_auto2)).
+    epose proof (H2 := @prf_equiv_congruence _ Γ 
+    _ _ {| pcEvar := x; pcPattern := ⌈ patt_free_evar x ⌉  |} ltac:(wf_auto2) H1).
+    cbn in H2. case_match. 2: congruence.
+    apply pf_iff_proj1 in H2. 2-3: wf_auto2.
+    mgAssert (⌈ patt_free_evar x and patt_free_evar y ⌉). wf_auto2.
+    mgClear 1. mgApplyMeta H2. mgExactn 0.
+    (* TODO: it is increadibly inconvienient to define concrete contexts *)
+    pose proof (@Singleton_ctx _ Γ 
+           (@ctx_app_r _ (patt_sym (Definedness_Syntax.inj definedness)) box 
+                ltac:(wf_auto2))
+           (@ctx_app_r _ (patt_sym (Definedness_Syntax.inj definedness)) box 
+                ltac:(wf_auto2)) (patt_free_evar y) x ltac:(wf_auto2)) as H3.
+    mgApplyMeta H3. simpl. mgSplitAnd. mgExactn 2. mgExactn 1.
+Defined.
